get_inv_up_iff

src/tree_of_strategy.lean
@@ -26,6 +26,21 @@ instance {n} : has_subset (Tree n) := ⟨(⊂ᵢ)⟩
 
 def branch {n} (η : Tree n) := { μ : Tree n // μ ⊂ᵢ η }
 
+lemma branch_linear {n} {η : Tree n} {μ₁ μ₂ : branch η} :
+  μ₂.val <:+ μ₁.val ↔ ¬μ₁.val ⊂ᵢ μ₂.val :=
+begin
+  split,
+  { simp[list.suffix_iff_is_initial], rintros (h | h),
+    { intros h₁, have := h.trans h₁, simp* at* },
+    { simp[h] } },
+  { simp[list.is_initial_iff_suffix], intros h,
+    rcases list.is_initial_iff_suffix.mp μ₁.property with ⟨h₁, eqn₁⟩,
+    rcases list.is_initial_iff_suffix.mp μ₂.property with ⟨h₂, eqn₂⟩,
+    have : μ₁.val <:+ μ₂.val ∨ μ₂.val <:+ μ₁.val, from list.suffix_or_suffix_of_suffix h₁ h₂,
+    cases this,
+    { simp[h this] }, { exact this } }
+end
+
 structure Tree_path (n : ℕ) :=
 (path : ℕ → Tree n)
 (ordered : ∀ m, path m <:+ path (m + 1))
@@ -79,6 +94,32 @@ lemma out_cons'_eq {n} {η : Tree n} (ν) (μ : branch η)  :
   @out n (ν :: η) μ.cons' = out μ :=
 by { simp[out, branch.cons'], intros h, exfalso, have := h μ.property, exact this }
 
+lemma out_cons'_eq' {n} {η : Tree n} (ν) (μ : branch η) {h : μ.val ⊂ᵢ ν :: η} :
+  @out n (ν :: η) ⟨μ.val, h⟩ = out μ :=
+by { simp[out, branch.cons'], intros h, exfalso, have := h μ.property, exact this }
+
+lemma suffix_out_eq {n} : ∀ {η₁ η₂: Tree n} {μ₁ : branch η₁} {μ₂ : branch η₂}
+  (h₁ : μ₁.val = μ₂.val) (h₂ : η₂ <:+ η₁), out μ₁ = out μ₂ :=
+begin
+  suffices : ∀ (l : list _) {η₁ η₂: Tree n} {μ₁ : branch η₁} {μ₂ : branch η₂}
+    (h₁ : μ₁.val = μ₂.val) (h₂ : l.reverse ++ η₂ = η₁), out μ₁ = out μ₂,
+  { intros η₁ η₂ μ₁ μ₂ h₁ h₂, rcases h₂ with ⟨l, h₂⟩,
+    exact this l.reverse h₁ (by simp[h₂]) },
+  intros l η₁ η₂ μ₁ μ₂ h₁ h₂,
+  induction l with ν l IH generalizing η₁ η₂,
+  { simp at h₂, rcases h₂ with rfl, congr, exact subtype.eq h₁ },
+  { simp at h₂,
+    let μ₂' : branch (ν :: η₂) := ⟨μ₂.val, μ₂.property.trans (by simp)⟩,
+    have h₁' : μ₁.val = μ₂'.val, { simp[μ₂', h₁] },
+    have eqn₁ : out μ₁ = out μ₂', from IH h₁' h₂,
+    have eqn₂ : out μ₂' = out μ₂, from out_cons'_eq' ν μ₂,
+    simp[eqn₁, eqn₂] }
+end
+
+lemma rnth_eq_iff_out {n} {η : Tree n} {μ : branch η} {ν} {m : ℕ} :
+  η.rnth m = some ν ↔ ν :: η↾*m <:+ η :=
+list.rnth_eq_iff_suffix_cons_initial
+
 namespace approx
 
 def weight (μ : Tree 1) : Π {η : Tree 0} (υ : branch η → option (Tree 1)), ℕ
@@ -105,44 +146,43 @@ lemma weight_pos_of {μ : Tree 1} : ∀ {η : Tree 0}
       { simp[weight], have := @weight_pos_of η (λ ν, υ ν.cons') ⟨⟨η₀.val, this⟩, by simp[branch.cons', h]⟩,
         exact nat.add_pos_left this _ } }
 
-def is_exists_inv_infinity (μ : Tree 1) :
+def get_inv_up (μ : Tree 1) :
   Π {η : Tree 0} (υ : branch η → option (Tree 1)), option (branch η)
 | []               _ := none
 | (sum.inl _ :: η) υ :=
-    if (@is_exists_inv_infinity η (λ ν, υ ν.cons')).is_some then
-      (@is_exists_inv_infinity η (λ ν, υ ν.cons')).map branch.cons' else
+    if (@get_inv_up η (λ ν, υ ν.cons')).is_some then
+      (@get_inv_up η (λ ν, υ ν.cons')).map branch.cons' else
     if υ ⟨η, by simp⟩ = ↑μ then some ⟨η, by simp⟩ else none
-| (sum.inr _ :: η) υ := (@is_exists_inv_infinity η (λ ν, υ ν.cons')).map branch.cons'
+| (sum.inr _ :: η) υ := (@get_inv_up η (λ ν, υ ν.cons')).map branch.cons'
 
 lemma is_some_of_out_infinity {η : Tree 1} :
   ∀ {μ : Tree 0} (υ : branch μ → option (Tree 1)) (μ₀ : branch μ)
-  (h1 : out μ₀ = ∞) (h2 : υ μ₀ = η), (is_exists_inv_infinity η υ).is_some 
+  (h1 : out μ₀ = ∞) (h2 : υ μ₀ = η), (get_inv_up η υ).is_some 
 | []       υ μ₀ _  _  := by { exfalso, have := μ₀.property, simp* at*  }
 | (ν :: μ) υ μ₀ h1 h2 :=
     begin
       have C₁ : μ₀.val = μ ∨ μ₀.val ⊂ᵢ μ, from list.is_initial_cons_iff.mp μ₀.property, cases C₁,
-      { cases ν; simp[is_exists_inv_infinity] at*,
+      { cases ν; simp[get_inv_up] at*,
         { cases ν,
-          cases C₂ : (@is_exists_inv_infinity η μ (λ ν, υ ν.cons')).is_some; simp[C₂],
-          { simp[←C₁, h2] },
-          { rcases option.is_some_iff_exists.mp C₂ with ⟨_, C₂⟩, simp[C₂] } },
+          cases C₂ : @get_inv_up η μ (λ ν, υ ν.cons'); simp[C₂],
+          { simp[←C₁, h2] } },
         { exfalso, have := out_eq_iff.mp h1, simp[←C₁] at this, exact this } },
-      { have IH : (is_exists_inv_infinity η (λ ν, υ ν.cons')).is_some,
+      { have IH : (get_inv_up η (λ ν, υ ν.cons')).is_some,
           from @is_some_of_out_infinity μ (λ ν, υ ν.cons') ⟨μ₀.val, C₁⟩
         (by {rw ←out_cons'_eq ν ⟨μ₀.val, C₁⟩, simp[branch.cons', h1] })
         (by simp[branch.cons', h2]),
-        cases ν; simp[is_exists_inv_infinity] at*; 
+        cases ν; simp[get_inv_up] at*; 
         rcases option.is_some_iff_exists.mp IH with ⟨_, IH⟩; simp[IH] }
     end
 
 lemma out_infinity_of_eq_some {η : Tree 1} :
   ∀ {μ : Tree 0} (υ : branch μ → option (Tree 1)) {μ₀ : branch μ}
-  (h : is_exists_inv_infinity η υ = some μ₀), out μ₀ = ∞ ∧ υ μ₀ = η
+  (h : get_inv_up η υ = some μ₀), out μ₀ = ∞ ∧ υ μ₀ = η
 | []               _ μ₀ _ := by { exfalso, have := μ₀.property, simp* at* }
 | (∞ :: μ)        υ μ₀ h :=
     begin
-      cases C₁ : (@is_exists_inv_infinity η μ (λ ν, υ ν.cons')).is_some;
-      simp[is_exists_inv_infinity, C₁] at h,
+      cases C₁ : (@get_inv_up η μ (λ ν, υ ν.cons')).is_some;
+      simp[get_inv_up, C₁] at h,
       { by_cases C₂ : υ ⟨μ, by simp⟩ = ↑η,
         { simp[C₂] at h,
           rcases h with rfl, simp[out_eq_iff, C₂] },
@@ -154,16 +194,83 @@ lemma out_infinity_of_eq_some {η : Tree 1} :
     end
 | (sum.inr ν :: μ) υ μ₀ h :=
     begin
-      simp[is_exists_inv_infinity] at h,
+      simp[get_inv_up] at h,
       rcases h with ⟨μ₁, h, eqn⟩,
         have IH : out μ₁ = ∞ ∧ υ μ₁.cons' = ↑η,
           from @out_infinity_of_eq_some _ (λ ν, υ ν.cons') μ₁ h,
       simp[←eqn, out_cons'_eq], exact IH
     end
 
+lemma get_inv_up_eq_some_of_eq_some (η : Tree 1) :
+  ∀ {μ : Tree 0} (υ : branch μ → option (Tree 1)) {μ₀ : branch μ} {μ₁ : branch μ₀.val}
+  (h : @get_inv_up η μ₀.val (λ x, υ ⟨x.val, x.property.trans μ₀.property⟩) = some μ₁),
+  get_inv_up η υ = some ⟨μ₁.val, μ₁.property.trans μ₀.property⟩
+| []       _ μ₀ _  _ := by { exfalso, have := μ₀.property, simp* at* }
+| (ν :: μ) υ μ₀ μ₁ h := 
+    begin
+      have C₁ : μ₀.val = μ ∨ μ₀.val ⊂ᵢ μ, from list.is_initial_cons_iff.mp μ₀.property, cases C₁,
+      { have : μ₀ = ⟨μ, by simp⟩, from subtype.ext_val C₁, rcases this with rfl,
+        { have : get_inv_up η (λ ν, υ ν.cons') = some μ₁, from h,
+          cases ν; simp[get_inv_up, this, h]; refl } },
+      have := @get_inv_up_eq_some_of_eq_some μ (λ ν, υ ν.cons') ⟨μ₀.val, C₁⟩ μ₁ h, 
+      cases ν; simp[get_inv_up, this, h]; refl
+    end
+
+private lemma get_inv_up_eq_none_of_eq_some {η : Tree 1} {μ : Tree 0} (υ : branch μ → option (Tree 1)) {μ₀ : branch μ}
+  (h : get_inv_up η υ = ↑μ₀) :
+  @get_inv_up η μ₀.val (λ x, υ ⟨x.val, x.property.trans μ₀.property⟩) = none :=
+begin
+  cases C : @get_inv_up η μ₀.val (λ x, υ ⟨x.val, x.property.trans μ₀.property⟩) with μ₁,
+  { refl },
+  exfalso,
+  have : get_inv_up η υ = some ⟨μ₁.val, _⟩, from get_inv_up_eq_some_of_eq_some η υ C,
+  have eqn : μ₁.val = μ₀.val, { simp[this] at h, exact congr_arg subtype.val (option.some_inj.mp h) },
+  have : μ₁.val ⊂ᵢ μ₀.val, from μ₁.property, 
+  simp [eqn] at this, exact this
+end
+
+lemma get_inv_up_iff
+  {η : Tree 1} {μ : Tree 0} (υ : branch μ → option (Tree 1)) {μ₀ : branch μ} :
+  (out μ₀ = ∞) ∧ (υ μ₀ = η) ∧ (∀ μ₁ : branch μ, out μ₁ = ∞ → υ μ₁ = η → μ₀.val <:+ μ₁.val) ↔
+  get_inv_up η υ = ↑μ₀ :=
+⟨λ ⟨h₁, h₂, h₃⟩,
+  begin
+    have : ∃ (μ₁ : branch μ), get_inv_up η υ = some μ₁,
+      from option.is_some_iff_exists.mp (is_some_of_out_infinity υ μ₀ h₁ h₂),
+    rcases this with ⟨μ₁, h_μ₁⟩,
+    have : out μ₁ = ∞ ∧ υ μ₁ = ↑η, from out_infinity_of_eq_some υ h_μ₁,
+    have lmm : μ₀.val <:+ μ₁.val := h₃ μ₁ this.1 this.2,
+    suffices : ¬ μ₀.val ⊂ᵢ μ₁.val,
+    { have : μ₀ = μ₁, from subtype.eq (list.suffix_antisymm lmm (branch_linear.mpr this)),
+      rw [this], exact h_μ₁ },
+    intros A,
+    have eqn : @get_inv_up η μ₁.val (λ x, υ ⟨x.val, x.property.trans μ₁.property⟩) = none,
+      from get_inv_up_eq_none_of_eq_some υ h_μ₁,
+    have : (@get_inv_up η μ₁.val (λ x, υ ⟨x.val, x.property.trans μ₁.property⟩)).is_some,
+    { have : out μ₀ = out ⟨μ₀.val, A⟩,
+        from @suffix_out_eq _ _ _ μ₀ ⟨μ₀.val, A⟩ rfl (list.suffix_of_is_initial μ₁.property),
+      refine is_some_of_out_infinity (λ x, υ ⟨x.val, x.property.trans μ₁.property⟩)
+      ⟨μ₀.val, A⟩ (by rw[←this, h₁]) (by simp; exact h₂) },
+    rw[eqn] at this, exact option.not_is_some_iff_eq_none.mpr rfl this
+  end, λ h,
+  begin
+    have := out_infinity_of_eq_some υ h,
+    refine ⟨this.1, this.2, λ μ₁ h₁ h₂, _⟩,
+    suffices : ¬ μ₁.val ⊂ᵢ μ₀.val,
+    { exact branch_linear.mpr this }, intros A,    
+    have eqn : @get_inv_up η μ₀.val (λ x, υ ⟨x.val, x.property.trans μ₀.property⟩) = none,
+      from get_inv_up_eq_none_of_eq_some υ h,
+    have : (@get_inv_up η μ₀.val (λ x, υ ⟨x.val, x.property.trans μ₀.property⟩)).is_some,
+    { have : out μ₁ = out ⟨μ₁.val, A⟩,
+        from @suffix_out_eq _ _ _ μ₁ ⟨μ₁.val, A⟩ rfl (list.suffix_of_is_initial μ₀.property),
+      refine is_some_of_out_infinity (λ x, υ ⟨x.val, x.property.trans μ₀.property⟩)
+      ⟨μ₁.val, A⟩ (by rw[←this, h₁]) (by simp; exact h₂) },
+    rw eqn at this, exact option.not_is_some_iff_eq_none.mpr rfl this
+  end⟩
+
 lemma out_neq_infinity_of_eq_none {η : Tree 1}
   {μ : Tree 0} (υ : branch μ → option (Tree 1))
-  (h : is_exists_inv_infinity η υ = none) (μ₀ : branch μ) : υ μ₀ = η → out μ₀ ≠ ∞ :=
+  (h : get_inv_up η υ = none) (μ₀ : branch μ) : υ μ₀ = η → out μ₀ ≠ ∞ :=
 begin
   by_cases C : υ μ₀ = ↑η ∧ out μ₀ = ∞,
   { exfalso, have := is_some_of_out_infinity υ μ₀ C.2 C.1, simp[h] at this, exact this },
@@ -172,16 +279,16 @@ end
 
 lemma eq_none_of_out_neq_infinity {η : Tree 1} :
   ∀ {μ : Tree 0} (υ : branch μ → option (Tree 1))
-  (h : ∀ μ₀ : branch μ, υ μ₀ = η → out μ₀ ≠ ∞), is_exists_inv_infinity η υ = none
-| []       _ _ := by simp[is_exists_inv_infinity]
+  (h : ∀ μ₀ : branch μ, υ μ₀ = η → out μ₀ ≠ ∞), get_inv_up η υ = none
+| []       _ _ := by simp[get_inv_up]
 | (ν :: μ) υ h :=
     begin
       have : ∀ (μ₀ : branch μ), υ μ₀.cons' = ↑η → out μ₀ ≠ ∞,
         { intros μ₀, simp[←out_cons'_eq ν μ₀, branch.cons'],
           have := h ⟨μ₀.val, μ₀.property.trans (μ.is_initial_cons _)⟩, exact this }, 
-        have : is_exists_inv_infinity η (λ ν, υ ν.cons') = none,
+        have : get_inv_up η (λ ν, υ ν.cons') = none,
           from eq_none_of_out_neq_infinity (λ ν, υ ν.cons') this,
-        cases ν; simp[is_exists_inv_infinity, this],
+        cases ν; simp[get_inv_up, this],
         { cases ν, intros hμ,
           have : out ⟨μ, _⟩ ≠ ∞ := h ⟨μ, by simp⟩ hμ,
           simp[out_eq_iff] at this, exact this }
@@ -191,7 +298,7 @@ def lambda' {η : Tree 0} (υ : branch η → option (Tree 1)) : ℕ → Tree 1
 | 0       := []
 | (n + 1) :=
     if 0 < weight (lambda' n) υ then
-      if h : (is_exists_inv_infinity (lambda' n) υ).is_some then
+      if h : (get_inv_up (lambda' n) υ).is_some then
         sum.inr (option.get h).val :: lambda' n
       else ∞ :: lambda' n
     else lambda' n
@@ -204,7 +311,7 @@ lemma lambda'_suffix_eq {η : Tree 0} (υ : branch η → option (Tree 1)) : ∀
     begin
       simp[lambda'] at h,
       by_cases C₁ : 0 < weight (lambda' υ n) υ; simp[C₁] at h,
-      { cases C₂ : (is_exists_inv_infinity (lambda' υ n) υ).is_some; simp[C₂] at h,
+      { cases C₂ : (get_inv_up (lambda' υ n) υ).is_some; simp[C₂] at h,
         { have C₃ : x :: μ = ∞ :: lambda' υ n ∨ x :: μ <:+ lambda' υ n, from list.suffix_cons_iff.mp h,
           cases C₃,
           { simp at C₃, refine ⟨n, lt_add_one n, by simp[C₃], by simp[lambda', C₁, C₂, C₃]⟩ },
@@ -228,7 +335,7 @@ begin
   { simp[out_eq_iff] at h, refine lambda'_suffix_eq υ h },
   rcases this with ⟨m, eqn_m, eqn_μ, eqn_μ'⟩,
   by_cases C₁ : 0 < weight (lambda' υ m) υ; simp[lambda', C₁] at eqn_μ',
-  { cases C₂ : is_exists_inv_infinity (lambda' υ m) υ with ν; simp[C₂] at eqn_μ',
+  { cases C₂ : get_inv_up (lambda' υ m) υ with ν; simp[C₂] at eqn_μ',
     { exfalso, have := list.head_eq_of_cons_eq eqn_μ', simp* at * },
     { have : ν.val = η₀,
         from sum.inr.inj (list.head_eq_of_cons_eq eqn_μ'),
@@ -239,33 +346,28 @@ begin
   exfalso, simp[eqn_μ] at eqn_μ', exact eqn_μ'
 end
 
-lemma out_infinity_of_out_neq_infinity
-  {η : Tree 0} (υ : branch η → option (Tree 1)) {n : ℕ} {μ : branch (lambda' υ n)}
-  (h₁ : ∃ η₀ : branch η, υ η₀ = μ.val) (h₂ : ∀ η₀ : branch η, υ η₀ = μ.val → out η₀ ≠ ∞) :
-  out μ = ∞ :=
-begin
-  have : ∃ m, m < n ∧ lambda' υ m = μ.val ∧ lambda' υ (m + 1) = out μ :: μ.val,
-    from lambda'_suffix_eq υ (suffix_out_cons μ),
-  rcases this with ⟨m, eqn_m, eqn_μ, eqn_μ'⟩,
-  have lmm₁ : 0 < weight μ.val υ, from weight_pos_of υ h₁,
-  have lmm₂ : is_exists_inv_infinity μ.val υ = none, from eq_none_of_out_neq_infinity υ h₂, simp at*,
-  simp[lambda', eqn_μ, lmm₁, lmm₂] at eqn_μ',
-  exact eq.symm (list.head_eq_of_cons_eq eqn_μ')
-end
-
-lemma out_neq_infinity_of_out_infinity {η : Tree 0} (υ : branch η → option (Tree 1)) {n : ℕ}
-  {μ : branch (lambda' υ n)} (h : out μ = ∞) :
-  (∃ η₀ : branch η, υ η₀ = μ.val) ∧ (∀ η₀ : branch η, υ η₀ = μ.val → out η₀ ≠ ∞) :=
-begin
-  have : ∃ m, m < n ∧ lambda' υ m = μ.val ∧ lambda' υ (m + 1) = ∞ :: μ.val,
-  { simp[out_eq_iff] at h, exact lambda'_suffix_eq υ h },
-  rcases this with ⟨m, eqn_m, eqn_μ, eqn_μ'⟩,
-  by_cases C₁ : 0 < weight (lambda' υ m) υ; simp[lambda', C₁] at eqn_μ',
-  { cases C₂ : is_exists_inv_infinity (lambda' υ m) υ with ν; simp[C₂] at eqn_μ',
-    { simp[←eqn_μ], refine ⟨of_weight_pos υ C₁, out_neq_infinity_of_eq_none υ C₂⟩ },
-    { exfalso, have := list.head_eq_of_cons_eq eqn_μ', simp* at* } },
-  { exfalso, simp[eqn_μ] at eqn_μ', exact eqn_μ' }
-end
+lemma out_neq_infinity_iff_out_infinity
+  {η : Tree 0} (υ : branch η → option (Tree 1)) {n : ℕ} {μ : branch (lambda' υ n)} :
+  (∃ η₀ : branch η, υ η₀ = μ.val) ∧ (∀ η₀ : branch η, υ η₀ = μ.val → out η₀ ≠ ∞) ↔ out μ = ∞ :=
+⟨λ ⟨h₁, h₂⟩, begin
+    have : ∃ m, m < n ∧ lambda' υ m = μ.val ∧ lambda' υ (m + 1) = out μ :: μ.val,
+      from lambda'_suffix_eq υ (suffix_out_cons μ),
+    rcases this with ⟨m, eqn_m, eqn_μ, eqn_μ'⟩,
+    have lmm₁ : 0 < weight μ.val υ, from weight_pos_of υ h₁,
+    have lmm₂ : get_inv_up μ.val υ = none, from eq_none_of_out_neq_infinity υ h₂, simp at*,
+    simp[lambda', eqn_μ, lmm₁, lmm₂] at eqn_μ',
+    exact eq.symm (list.head_eq_of_cons_eq eqn_μ')
+  end, λ h,
+  begin
+    have : ∃ m, m < n ∧ lambda' υ m = μ.val ∧ lambda' υ (m + 1) = ∞ :: μ.val,
+    { simp[out_eq_iff] at h, exact lambda'_suffix_eq υ h },
+    rcases this with ⟨m, eqn_m, eqn_μ, eqn_μ'⟩,
+    by_cases C₁ : 0 < weight (lambda' υ m) υ; simp[lambda', C₁] at eqn_μ',
+    { cases C₂ : get_inv_up (lambda' υ m) υ with ν; simp[C₂] at eqn_μ',
+      { simp[←eqn_μ], refine ⟨of_weight_pos υ C₁, out_neq_infinity_of_eq_none υ C₂⟩ },
+      { exfalso, have := list.head_eq_of_cons_eq eqn_μ', simp* at* } },
+    { exfalso, simp[eqn_μ] at eqn_μ', exact eqn_μ' }
+  end⟩
 
 def lambda {η : Tree 0} (υ : branch η → option (Tree 1)) : Tree 1 := lambda' υ η.length
 
@@ -315,6 +417,11 @@ lemma out_neq_infinity_of_out_infinity {η : Tree 0} {μ : branch (S.lambda η)}
 (approx.out_neq_infinity_of_out_infinity (up' S η) h).2 η₀
 (by { simp[up'_up_consistent], exact up })
 
+lemma out_neq_infinity_of_out_infinity {η : Tree 0} {μ : branch (S.lambda η)} {η₀ : Tree 0}
+  (h : out μ = sum.inr η₀) : ∃ h : η₀ ⊂ᵢ η, out ⟨η₀, h⟩ = ∞ ∧ S.up η₀ = μ.val :=
+(approx.out_neq_infinity_of_out_infinity (up' S η) h).2 η₀
+(by { simp[up'_up_consistent], exact up })
+
 variables (Λ : Tree_path 0)
 
 theorem finite_injury :
@@ -328,17 +435,19 @@ begin
       ∃ s₁, s₀ ≤ s₁ ∧ ∀ s, s₁ ≤ s → (S.lambda (Λ.path s)).rnth n = (S.lambda (Λ.path s₁)).rnth n,
     { rcases this with ⟨s₁, eqn, hyp_s₁⟩, refine ⟨s₁, λ s eqn_s, _⟩,
       apply list.rnth_ext', { intros m a, simp[list.initial_rnth_some_iff], sorry } },
-    by_cases C₁ : ∀ s, list.rnth (S.lambda (Λ.path s)) n = none,
+    by_cases C₁ : ∀ s, (S.lambda (Λ.path s)).rnth n = none,
     { refine ⟨s₀, by refl, λ s eqn_s, _⟩, simp[C₁] },
-    have C₁ : ∃ (s₁ : ℕ) (ν : infinity ⊕ Tree 0), list.rnth (S.lambda (Λ.path s₁)) n = some ν,
+    have C₁ : ∃ s₁ ν, (S.lambda (Λ.path s₁)).rnth n = some ν,
     { simp at C₁, rcases C₁ with ⟨s₁, C₁⟩, have := option.ne_none_iff_exists'.mp C₁, exact ⟨s₁, this⟩ },
     rcases C₁ with ⟨s₁, ν, C₁⟩,
     cases ν,
-    { cases ν, refine ⟨max s₀ s₁, by simp, λ s eqn_s, _⟩,
+    { cases ν,
+      
+      
         } }
 
 end 
-
+--/
 end strategy
 
 
